src/case_study/examples.v
@@ -56,12 +56,12 @@ Section stack_lang_examples.
   Proof.
     iIntros (Φ) "Hsize #HΦ /=". rewrite /example1. prepare_ctx.
     iApply wp_call_global;[eauto|iFrame]. iNext. iIntros "Hsize /=". prepare_ctx.
-    iApply wp_stack_alloc;[lia|repeat constructor|iFrame].
+    iApply wp_stack_alloc;[repeat constructor|iFrame].
     iNext. iIntros (l) "[Hsize Hl]". peel_ctx.
     iApply wp_LetIn. iIntros "!>". simpl subst'.
-    iApply wp_stack_load;[constructor;lia|iFrame].
+    iApply (wp_stack_load);[|iFrame];[eauto|].
     iNext. iIntros "[Hsize Hl]". peel_ctx.
-    iApply wp_return;[lia..|iFrame]. iNext. iIntros "Hsize".
+    iApply wp_return;[eauto|lia|iFrame]. iNext. iIntros "Hsize".
     iModIntro.
     simpl. iApply wp_value. iApply "HΦ". simpl. auto.
   Qed.
@@ -71,17 +71,17 @@ Section stack_lang_examples.
   Proof.
     iIntros (Φ) "Hsize #HΦ /=". rewrite /example2. prepare_ctx.
     iApply wp_call_global;[eauto|iFrame]. iIntros "!>". iIntros "Hsize /=". prepare_ctx.
-    iApply wp_stack_alloc;[lia|repeat constructor|iFrame].
+    iApply wp_stack_alloc;[repeat constructor|iFrame].
     iNext. iIntros (l) "[Hsize Hl]". peel_ctx.
     iApply wp_LetIn. iIntros "!>". simpl subst'.
     iApply wp_call_global;[eauto|iFrame]. iNext. iIntros "Hsize /=".
     prepare_ctx.
-    iApply wp_stack_load;[constructor;lia|iFrame].
+    iApply wp_stack_load;[|iFrame];eauto.
     iNext. iIntros "[Hsize Hl]". peel_ctx.
-    iApply wp_return;[lia..|iFrame]. iNext. iIntros "Hsize /=".
+    iApply wp_return;[eauto|lia|iFrame]. iNext. iIntros "Hsize /=".
     iDestruct (stack_stack_pop_intro with "Hl") as "Hl";[eauto|].
     iModIntro. prepare_ctx.
-    iApply wp_return;[lia..|iFrame]. iNext. iClear "Hl".
+    iApply wp_return;[eauto|lia..|iFrame]. iNext. iClear "Hl".
     iIntros "Hsize /=". iClear "Hsize". iModIntro.
     iApply wp_value. iApply "HΦ";auto.
   Qed.
@@ -93,21 +93,21 @@ Section stack_lang_examples.
     iApply wp_LetIn. iIntros "!>". simpl subst'.
     iApply wp_LetIn. iIntros "!>". simpl subst'.
     iApply wp_call_global;[eauto|iFrame]. iNext. iIntros "Hsize /=". prepare_ctx.
-    iApply wp_stack_alloc;[lia|repeat constructor|iFrame]. iNext. iIntros (l) "[Hsize Hl]". peel_ctx.
+    iApply wp_stack_alloc;[repeat constructor|iFrame]. iNext. iIntros (l) "[Hsize Hl]". peel_ctx.
     iApply wp_LetIn. iIntros "!>". simpl subst'.
     iApply wp_call_global;[eauto|iFrame]. iNext. iIntros "Hsize /=". prepare_ctx.
-    iApply wp_call_local;[eauto..|iFrame];[constructor;lia|]. simpl. prepare_ctx.
+    iApply wp_call_local;[eauto..|iFrame]. simpl. prepare_ctx.
     iNext. iIntros "Hsize".
     (* NOTE: the local stack pointer has been shifted to point two frame down *)
-    iApply wp_stack_load;[constructor;lia|iFrame]. iNext. iIntros "[Hsize Hl]". peel_ctx.
-    iApply wp_return;[lia..|]. iFrame. iNext.
+    iApply wp_stack_load;[|iFrame];eauto. iNext. iIntros "[Hsize Hl]". peel_ctx.
+    iApply wp_return;[eauto|lia|]. iFrame. iNext.
     iIntros "Hsize /=".
     iDestruct (stack_stack_pop_intro _ _ _ _ 2 with "Hl") as "Hl";[lia|].
     iModIntro. prepare_ctx.
-    iApply wp_return;[lia..|]. iFrame. iNext. iIntros "Hsize /=".
+    iApply wp_return;[eauto|lia|]. iFrame. iNext. iIntros "Hsize /=".
     iDestruct (stack_stack_pop_intro _ _ _ _ 1 with "Hl") as "Hl";[lia|].
     iModIntro. prepare_ctx.
-    iApply wp_return;[lia..|]. iFrame. iNext. iIntros "Hsize /=".
+    iApply wp_return;[eauto|lia..|]. iFrame. iNext. iIntros "Hsize /=".
     iClear "Hl".
     iModIntro. iApply wp_value. iApply "HΦ";auto.
   Qed.
@@ -120,8 +120,8 @@ Section stack_lang_examples.
   Proof.
     iIntros (Φ) "Hsize #HΦ /=". rewrite /stuck_example. prepare_ctx.
     iApply wp_call_global;[eauto|iFrame]. iNext. iIntros "Hsize /=". prepare_ctx.
-    iApply wp_stack_alloc;[lia|repeat constructor|iFrame]. iNext. iIntros (l) "[Hsize Hl]". peel_ctx.
-    iApply wp_return;[lia..|iFrame]. iNext. iIntros "Hsize /=". iModIntro.
+    iApply wp_stack_alloc;[repeat constructor|iFrame]. iNext. iIntros (l) "[Hsize Hl]". peel_ctx.
+    iApply wp_return;[eauto|lia|iFrame]. iNext. iIntros "Hsize /=". iModIntro.
     (* STUCK! the points-to for l gets lost, its lifetime is not less than 1 *)
   Abort.
 
@@ -130,10 +130,10 @@ Section stack_lang_examples.
   Lemma example4_spec (e : expr) :
     (forall v, expr_subst "f" v e = e) -> (* e does not contain free f *)
     (∀ (j : nat) v1 v2 K', {{{ [size] j
-                      ∗ (∃ (i : nat) K (off : Z), ⌜(off <= 0)%Z⌝ ∧ ⌜shift_expr v2 (-1) = Cont off K⌝ ∧ ⌜(i = j + 1 - (Z.abs_nat off))⌝ ∧
+                      ∗ (∃ (i : nat) K (off : nat), ⌜(off ≤ j)⌝ ∧ ⌜shift_expr v2 (-1) = Some (Cont off K)⌝ ∧ ⌜(i = j - off)⌝ ∧
                                       (∀ v', (∃ n, ⌜v' = Nat n⌝) → [size] i -∗
                                       ⚡={Ω <- (lifetime_stack i)}=> WP fill K (i,v') {{ λ v, ∃ n, ⌜v.2 = NatV n⌝ }}))
-                      ∗ (∃ i l (off : Z), ⌜(off <= 0)%Z⌝ ∧ ⌜shift_expr v1 (-1) = Loc (local off) l⌝ ∧ ⌜(i = j - (Z.abs_nat off))⌝ ∧
+                      ∗ (∃ i l (off : nat), ⌜(off <= j)⌝ ∧ ⌜shift_expr v1 1 = Some (Loc (local off) l)⌝ ∧ ⌜(i = j - (Z.abs_nat off))⌝ ∧
                                       inv (logN .@ l) (lifetime_stack i) (∃ v, i @@ l ↦ v ∗ ∃ m, ⌜v = NatV m⌝))
                       ∗ (∀ v', (∃ n, ⌜v' = Nat n⌝) → [size] j -∗
                         ⚡={Ω <- (lifetime_stack j)}=> WP fill K' (j,v') {{ λ v, ∃ n, ⌜v.2 = NatV n⌝ }}) }}}
@@ -145,7 +145,7 @@ Section stack_lang_examples.
     iModIntro. iIntros (Φ) "Hsize #HΦ /=". rewrite /example4. prepare_ctx.
     iApply wp_LetIn. iIntros "!>". simpl subst'.
     iApply wp_call_global;[eauto|iFrame]. iIntros "!> Hsize". prepare_ctx.
-    iApply wp_stack_alloc;[lia|repeat constructor|iFrame]. iIntros "!>" (l) "[Hsize Hl] /=". prepare_ctx.
+    iApply wp_stack_alloc;[repeat constructor|iFrame]. iIntros "!>" (l) "[Hsize Hl] /=". prepare_ctx.
     iApply wp_LetIn. iIntros "!> /=".
     prepare_ctx. rewrite Hfree. iApply fupd_wp.
     iMod (@inv_alloc _ _ _ _ locality_lifetime_pick _ (logN .@ l) _
@@ -159,7 +159,7 @@ Section stack_lang_examples.
     iApply ("Hadv_spec" with "[-] [//]"). iFrame.
     iSplitR;[|iSplitR].
     - (* the unknown function returns to the first caller *)
-      iExists 0,[],(-2)%Z.
+      iExists 1,[],0.
       iSplit;[iPureIntro;lia|].
       iSplit;[auto|].
       iSplit;[iPureIntro;lia|].
@@ -167,7 +167,7 @@ Section stack_lang_examples.
       iClear "Hinv Hadv_spec". iModIntro.
       destruct Hv' as [? ->]. simpl. iApply wp_value;eauto.
     - (* invariant for the stack variable parameter *)
-      iExists 0,l,(-1)%Z.
+      iExists 0,l,1.
       iSplit;[iPureIntro;lia|].
       iSplit;[auto|].
       iSplit;[iPureIntro;lia|].
@@ -185,11 +185,11 @@ Section stack_lang_examples.
       { unfold SameGeneration. by cbn. }
       iMod (inv_acc with "Hinv") as "[>Hl Hcls]";[set_solver|].
       iDestruct "Hl" as (v) "[Hl %Heq]". destruct Heq as [? ->].
-      iModIntro. prepare_ctx. iApply wp_stack_load;[repeat constructor;lia|].
+      iModIntro. prepare_ctx. iApply wp_stack_load;[|iFrame];eauto.
       iFrame. iIntros "!> [Hsize Hl] /=".
       iApply wp_value. iMod ("Hcls" with "[Hl]") as "_";[eauto|].
       iModIntro. prepare_ctx.
-      iApply wp_return;[lia|lia|]. iFrame.
+      iApply wp_return;[eauto|lia|]. iFrame.
       iIntros "!> Hsize". iClear "Hinv". iModIntro.
       simpl. iApply wp_value. eauto.
   Qed.
